{"nbformat":4,"nbformat_minor":0,"metadata":{"colab":{"provenance":[],"authorship_tag":"ABX9TyN/dDkl9lAkbVZAFZ0aF56H"},"kernelspec":{"name":"python3","display_name":"Python 3"},"language_info":{"name":"python"}},"cells":[{"cell_type":"markdown","source":["Your task is to create a function called sum_arrays(), which takes two arrays consisting of integers, and returns the sum of those two arrays.\n","\n","The twist is that (for example) [3,2,9] does not equal 3 + 2 + 9, it would equal '3' + '2' + '9' converted to an integer for this kata, meaning it would equal 329. The output should be an array of the sum in a similar fashion to the input (for example, if the sum is 341, you would return [3,4,1]). Examples are given below of what two arrays should return.\n","\n","[3,2,9],[1,2] --> [3,4,1]\n","\n","[4,7,3],[1,2,3] --> [5,9,6]\n","\n","[1],[5,7,6] --> [5,7,7]\n","\n","If both arrays are empty, return an empty array.\n","\n","In some cases, there will be an array containing a negative number as the first index in the array. In this case treat the whole number as a negative number. See below:\n","\n","[3,2,6,6],[-7,2,2,8] --> [-3,9,6,2] # 3266 + (-7228) = -3962"],"metadata":{"id":"IcF5QpFPDmzY"}},{"cell_type":"code","execution_count":null,"metadata":{"id":"2RtU_Gl7DViw"},"outputs":[],"source":["def sum_arrays(array1,array2):\n","    x=11\n","    arr1=\"\"\n","    arr2=\"\"\n","    result=[]\n","    if (len(array1) > 0) & (len(array2) > 0):\n","        for i in array1:\n","            arr1+=f\"{i}\"\n","        for k in array2:\n","            arr2+=f\"{k}\"\n","        sum = int(arr1) + int(arr2)\n","        sum=str(sum)\n","        for i in sum:\n","            if i != \"-\":\n","                result.append(int(i))\n","            else:\n","                result.append(i)\n","        if result[0]=='-':\n","            del result[0]\n","            result[0]=-result[0]\n","        if (result[0] == 0) & (len(result) != 0) & (result !=[0]):\n","            del result[0]\n","        return result\n","    elif (len(array1) ==0) & (len(array2) ==0):\n","        return []\n","    elif len(array1) == 0:\n","        if array2 !=[0]:\n","            while(array2[0]==0):\n","                del array2[0]\n","                if len(array2)==0:\n","                    break\n","        return array2\n","    elif len(array2) == 0:\n","        if array1 !=[0]:\n","            while(array1[0]==0):\n","                del array1[0]\n","                if len(array1)==0:\n","                    break\n","        return array1\n","sum_arrays([0] , [0])"]}]}